state/Monotonic.IFC.Heap.fsti
@@ -263,3 +263,12 @@ val lemma_next_addr_alloc
 val lemma_next_addr_contained_refs_addr
   (#a:Type0) (#rel:preorder a) (h:lheap) (r:mref a rel)
   :Lemma (h `contains` r ==> addr_of r < next_addr h)
+
+val lemma_alloc_props
+  (#a:Type0) (#rel:preorder a) (h0:lheap) (x:a) (mm:bool)
+  :Lemma (
+    let rh1 = alloc rel h0 x mm in 
+    label_of (fst rh1) (snd rh1) == High /\
+    modifies_classification Set.empty h0 (snd rh1) /\
+    (forall (a:Type0) (rel:preorder a) (r:mref a rel). 
+      h0 `contains` r ==> label_of r h0 `label_gte` label_of r (snd rh1)))
